src/named/SimpleEvalCtx.v
@@ -12,96 +12,83 @@ Import Core.Notations.
 Require Coq.derive.Derive.
 
 
-Definition subst_eval_ctx :=
-  [(* TODO: do I want a substitution eval ctx? I think no
-         [:> "G1" : #"env", "G2" : #"env", "G3" : #"env", "f" : #"sub" %"G1" %"G2", "g" : #"sub" %"G2" %"G3", "A" : #"ty", "e" : #"el" %"G3" %"A"
-        ----------------------------------------------- ("el_subst_cmp")
-        #"el_subst" %"f" (#"el_subst" %"g" %"e") = #"el_subst" (#"cmp" %"f" %"g") %"e" : #"el" %"G1" %"A"
-    ]%arule;
-  [:> "G" : #"env", "A" : #"ty", "B": #"ty", "E" : #"Ectx" %"G'" %"A" %"B"
-        ----------------------------------------------- ("E_subst_id")
-        #"E_subst" #"id" %"E" = %"E" : #"Ectx" %"G'" %"A" %"B"
-    ]%arule;
-  [:| "G" : #"env", "G'" : #"env", "g" : #"sub" %"G" %"G'",
-      "A" : #"ty", "B" : #"ty", "E" : #"Ectx" %"G" %"A" %"B"
-        -----------------------------------------------
-        #"E_subst" "g" "E" : #"Ectx" %"G'" %"A" %"B"
-    ];*)
-     [:> "G" : #"env", "A" : #"ty",
-         "e" : #"el" %"G" %"A"
-        ----------------------------------------------- ("plug hole")
-        #"plug" #"[ ]" %"e" = %"e" : #"el" %"G" %"A"
-     ];
-     [:| "G" : #"env", "A" : #"ty", "B" : #"ty",
-         "E" : #"Ectx" %"G" %"A" %"B",
-         "e" : #"el" %"G" %"A"
-        -----------------------------------------------
-        #"plug" "E" "e" : #"el" %"G" %"B"
-     ];
-     [:| "G" : #"env", "A" : #"ty"
-        -----------------------------------------------
-        #"[ ]" : #"Ectx" %"G" %"A" %"A"
-     ];
-     [s| "G" : #"env", "A" : #"ty", "B" : #"ty"
-        -----------------------------------------------
-        #"Ectx" "G" "A" "B" srt
-     ]
-  ]%arule.
-
-Derive eval_ctx_elab
-       SuchThat (Pre.elab_lang subst_elab subst_eval_ctx eval_ctx_elab)
+Definition subst_eval_ctx_def : lang :=
+  {[l
+  [s| "G" : #"env", "A" : #"ty", "B" : #"ty"
+      -----------------------------------------------
+      #"Ectx" "G" "A" "B" srt
+  ];
+  [:| "G" : #"env", "A" : #"ty"
+      -----------------------------------------------
+      #"[ ]" : #"Ectx" "G" "A" "A"
+  ];       
+  [:| "G" : #"env", "A" : #"ty", "B" : #"ty",
+      "E" : #"Ectx" "G" "A" "B",
+      "e" : #"exp" "G" "A"
+      -----------------------------------------------
+      #"plug" "E" "e" : #"exp" "G" "B"
+  ];
+  [:= "G" : #"env", "A" : #"ty",
+      "e" : #"exp" "G" "A"
+      ----------------------------------------------- ("plug hole")
+      #"plug" #"[ ]" "e" = "e" : #"exp" "G" "A"
+  ]]}.
+       
+Derive eval_ctx
+       SuchThat (Pre.elab_lang (exp_subst ++ value_subst) subst_eval_ctx_def eval_ctx)
        As eval_ctx_wf.
 Proof. auto_elab. Qed.
 #[export] Hint Resolve eval_ctx_wf : elab_pfs.
 
 
-Definition Estlc :=  
-  [
-     [:> "G" : #"env",
-       "A" : #"ty",
-       "B" : #"ty",
-       "C" : #"ty",
-       "E" : #"Ectx" %"G" %"C" %"A",
-       "v" : #"val" %"G" (#"->" %"A" %"B"),
-       "e" : #"el" %"G" %"C"
-       ----------------------------------------------- ("plug app_r")
-       #"plug" (#"Eapp_r" %"v" %"E") %"e"
-       = #"app" (#"ret" %"v") (#"plug" %"E" %"e")
-      : #"el" %"G" %"B"
+Definition Estlc_def :lang :=  
+  {[l
+  [:| "G" : #"env",
+      "A" : #"ty",
+      "B" : #"ty",
+      "C" : #"ty",
+      "E" : #"Ectx" "G" "C" (#"->" "A" "B"),
+      "e'" : #"exp" "G" "A"
+      -----------------------------------------------
+      #"Eapp_l" "E" "e'" : #"Ectx" "G" "C" "B"
   ];
-     [:| "G" : #"env",
+  [:= "G" : #"env",
        "A" : #"ty",
        "B" : #"ty",
        "C" : #"ty",
-       "v" : #"val" %"G" (#"->" %"A" %"B"),
-       "E" : #"Ectx" %"G" %"C" %"A"
-       -----------------------------------------------
-       #"Eapp_r" "v" "E" : #"Ectx" %"G" %"C" %"B"
-  ];
-     [:> "G" : #"env",
-       "A" : #"ty",
-       "B" : #"ty",
-       "C" : #"ty",
-       "E" : #"Ectx" %"G" %"C" (#"->" %"A" %"B"),
-       "e'" : #"el" %"G" %"A",
-       "e" : #"el" %"G" %"C"
+       "E" : #"Ectx" "G" "C" (#"->" "A" "B"),
+       "e'" : #"exp" "G" "A",
+       "e" : #"exp" "G" "C"
        ----------------------------------------------- ("plug app_l")
-       #"plug" (#"Eapp_l" %"E" %"e'") %"e"
-       = #"app" (#"plug" %"E" %"e") %"e'"
-      : #"el" %"G" %"B"
+       #"plug" (#"Eapp_l" "E" "e'") "e"
+       = #"app" (#"plug" "E" "e") "e'"
+      : #"exp" "G" "B"
   ];
-     [:| "G" : #"env",
+  [:| "G" : #"env",
        "A" : #"ty",
        "B" : #"ty",
        "C" : #"ty",
-       "E" : #"Ectx" %"G" %"C" (#"->" %"A" %"B"),
-       "e'" : #"el" %"G" %"A"
+       "v" : #"val" "G" (#"->" "A" "B"),
+       "E" : #"Ectx" "G" "C" "A"
        -----------------------------------------------
-       #"Eapp_l" "E" "e'" : #"Ectx" %"G" %"C" %"B"
-  ]]%arule.
+       #"Eapp_r" "v" "E" : #"Ectx" "G" "C" "B"
+  ];
+  [:= "G" : #"env",
+      "A" : #"ty",
+      "B" : #"ty",
+      "C" : #"ty",
+      "E" : #"Ectx" "G" "C" "A",
+      "v" : #"val" "G" (#"->" "A" "B"),
+      "e" : #"exp" "G" "C"
+      ----------------------------------------------- ("plug app_r")
+      #"plug" (#"Eapp_r" "v" "E") "e"
+      = #"app" (#"ret" "v") (#"plug" "E" "e")
+      : #"exp" "G" "B"
+  ]]}.
 
-Derive Estlc_elab
-       SuchThat (Pre.elab_lang (eval_ctx_elab ++ stlc_elab ++ subst_elab) Estlc Estlc_elab)
+
+Derive Estlc
+       SuchThat (Pre.elab_lang (eval_ctx ++ stlc ++ exp_subst++ value_subst) Estlc_def Estlc)
        As Estlc_wf.
 Proof. auto_elab. Qed.
 #[export] Hint Resolve Estlc_wf : elab_pfs.
