src/named/SimpleUnit.v
@@ -12,23 +12,23 @@ Import Core.Notations.
 Require Coq.derive.Derive.
 
 Definition unit_lang_def : lang :=
-  [[l
+  {[l
   [:|
      -----------------------------------------------
       #"unit" : #"ty"
   ];
   [:| "G" : #"env"
       -----------------------------------------------
-      #"tt" : #"val" %"G" #"unit"
+      #"tt" : #"val" "G" #"unit"
     ];
-  [:> "G" : #"env",
+  [:= "G" : #"env",
       "G'" : #"env",
-      "g" : #"sub" %"G'" %"G"
+      "g" : #"sub" "G'" "G"
       ----------------------------------------------- ("tt_subst")
-      #"val_subst" %"g" #"tt" = #"tt"
-      : #"val" %"G'" #"unit"
+      #"val_subst" "g" #"tt" = #"tt"
+      : #"val" "G'" #"unit"
   ]
-  ]].
+  ]}.
 
 
 Derive unit_lang
@@ -38,12 +38,12 @@ Proof. auto_elab. Qed.
 #[export] Hint Resolve unit_wf : elab_pfs.
 
 Definition unit_eta_def :lang :=
-  [[l [:> "G" : #"env",
-       "v" : #"val" %"G" #"unit"
+  {[l [:= "G" : #"env",
+       "v" : #"val" "G" #"unit"
       ----------------------------------------------- ("unit eta")
-      %"v" = #"tt"
-      : #"val" %"G" #"unit"
-  ] ]].
+      "v" = #"tt"
+      : #"val" "G" #"unit"
+  ] ]}.
 
 
 Derive unit_eta
